Adding hypotheses to the context

website/Walkthrough/Blog/AddingGoalsAndHypotheses.lean
@@ -5,7 +5,6 @@ open Verso Genre Blog
 #doc (Page) "Adding goals and hypotheses" =>
 
 ```leanInit AGH
-open Lean Meta Elab Tactic
 ```
 
 By the end of this section, you'll create a version of the `apply` tactic.
@@ -19,6 +18,8 @@ We've seen before that `getMainGoal` gives us the details of the current goal. T
 Here is a tactic that lets us test this out.
 
 ```lean AGH
+open Lean Meta Elab Tactic
+
 elab "print_goals" : tactic => do
   let goals ← getUnsolvedGoals
   for goal in goals do
@@ -73,7 +74,7 @@ We can extract out the basics of goal creation into a helper tactic: `createGoal
 ```lean AGH
 open Lean Elab Meta Tactic
 
-def createGoal (goalType : Expr) : TacticM Unit := do
+def createGoal (goalType : Expr) : TacticM Unit := withMainContext do
   let goal ← mkFreshExprMVar goalType
   appendGoals [goal.mvarId!]
 ```
@@ -109,15 +110,105 @@ example : 1 + 2 = 3 := by
 We can also modify the syntax of the tactic to include the type of the new goal as a parameter.
 
 ```lean AGH
-elab "create_goal_of" t:term : tactic => do
+elab "create_goal" t:term : tactic => do
   let e ← Term.elabTerm t none
   createGoal e
 
 example : 1 + 2 = 3 := by
-  create_goal_of (Nat.Prime 2)
+  create_goal (Nat.Prime 2)
   simp; exact Nat.prime_two
 ```
 
 # Adding a new hypothesis
 
 Similarly, we can extract out the basics of hypothesis creation into a helper tactic: `createHypothesis`.
+
+```lean AGH
+def createHypothesis (hypType : Expr) (hypProof : Expr) (hypName := `h) : TacticM Unit := do
+  let hyp : Hypothesis := { userName := hypName, type := hypType, value := hypProof }
+  let (_, new_goal) ← (← getMainGoal).assertHypotheses (List.toArray [hyp])
+  setGoals [new_goal]
+```
+
+Here’s an example of adding a hypothesis that looks like `h : ℕ`.
+
+```lean AGH
+elab "create_nat_hypothesis" : tactic => do
+  let hypType := Expr.const ``Nat []
+  let hypProof := (toExpr 0) -- use 0 as a term of type Nat
+  createHypothesis hypType hypProof
+
+example : 1 + 2 = 3 := by
+  create_nat_hypothesis
+  simp
+```
+
+Here’s an example of adding a hypothesis that is a proposition `0 = 0`.
+
+```
+elab "create_reflexivity_hypothesis" : tactic => do
+  let hypType ← mkEq (toExpr 0) (toExpr 0) -- make the metavariable goal to prove that "0 = 0"
+  let hypProof ← mkAppM ``Eq.refl #[toExpr 0] -- proof that Eq 0 0
+  createHypothesis hypType hypProof
+
+example : 1 + 2 = 3 := by
+  create_reflexivity_hypothesis
+  simp
+```
+
+# Catching errors when adding a hypothesis
+
+Lean will technically let us create bogus hypotheses.
+
+```lean AGH
+elab "create_bogus_hypothesis" : tactic => do
+  let hypType ← mkEq (toExpr 0) (toExpr 1) -- make the metavariable goal to prove that "0 = 0"
+  let hypProof  ← mkAppM ``Eq.refl #[toExpr 0] -- proof that Eq 0 0
+  createHypothesis hypType hypProof
+```
+
+```lean AGH
+example : 0=1 := by
+  create_bogus_hypothesis -- a new bogus hypothesis in the context
+  sorry
+```
+But, if we actually try to use that hypothesis to prove a theorem, it will throw an error
+
+```lean AGH error:=true
+example : 0=1 := by
+  create_bogus_hypothesis
+  assumption
+```
+
+The issue here is that the tactic isn't checking the hypothesis statement matches the proof …
+
+That is, by propositions-as-types and proofs-as-terms, the inferred type of the proof should be the type.
+
+A similar thing occurred previously with `setGoals`, where we could drop all active goals from the tactic state.
+
+So let's modify our `createHypothesis` function to check that ...
+
+```lean AGH
+def createHypothesisGuarded (hypType : Expr) (hypProof : Expr) : TacticM Unit := do
+  let hypName := `h
+  unless ← isDefEq hypType (← inferType hypProof) do
+    throwError "The proof used for creating the hypothesis does not match the expected type."
+  let hyp : Hypothesis := { userName := hypName, type := hypType, value := hypProof }
+  let (_, new_goal) ← (← getMainGoal).assertHypotheses (List.toArray [hyp])
+  setGoals [new_goal]
+```
+
+Here, the `inferType` function is used to deduce the type of `hypProof` (or the statement of the theorem it is a proof of, in the case of propositions). The `isDefEq` function is used to compare two expressions up to definitional equality; more will be said about this function in the later sections.
+
+Adding the bogus hypothesis no longer works with the `createHypothesisGuarded` function.
+
+```lean AGH error := true
+elab "create_bogus_hypothesis" : tactic => do
+  let hypType ← mkEq (toExpr 0) (toExpr 1) -- make the metavariable goal to prove that "0 = 0"
+  let hypProof  ← mkAppM ``Eq.refl #[toExpr 0] -- proof that Eq 0 0
+  createHypothesisGuarded hypType hypProof
+
+example : 0=1 := by
+  create_bogus_hypothesis
+  assumption
+```
